Work on hnf

proof/Hnf.v
@@ -6,29 +6,61 @@ Require Import Lambda.Env.
 
 Set Implicit Arguments.
 
-Implicit Types i k m n p : nat.
+Implicit Types i k m n : nat.
 Implicit Type s : sort.
 Implicit Types A B M N T t u v : term.
 
-Definition redex (x : term) :=
+Fixpoint redex (x : term) :=
   match x with
   App (Abs _ _) _ => True
   | Pi1 (Pair _ _ _) => True
   | Pi2 (Pair _ _ _) => True
+  | App x y => redex x 
+  | Pi1 x => redex x
+  | Pi2 x => redex x
   | _ => False
   end.
 
+Axiom hnf_measure : term -> nat.
+
+Program Fixpoint hnf (x : term) { measure x hnf_measure } : term :=
+  match x with
+  | App x y => 
+    match hnf x with
+    | Abs T v => hnf (subst y v)
+    | h => App h y
+    end
+  | Pi1 x =>
+    match hnf x with
+    | Pair T u v => hnf u
+    | h => Pi1 h
+    end
+  | Pi2 x =>
+    match hnf x with
+    | Pair T u v => hnf u
+    | h => Pi2 h
+    end
+  | x => x
+  end.
+
+Obligation 1.
+  simpl ; subst ; intros.
+  subst.
+
+
 Inductive hnf : term -> term -> Prop :=
-  | hnf_beta : forall T e v, 
+  | hnf_beta : forall x, forall T e v, 
+    (hnf x (Abs T e) -> 
     forall H, hnf (subst v e) H ->
-    hnf (App (Abs T e) v) H
-  | hnf_pi1 :  forall T x y, 
+    hnf (App x v) H) ->
+    
+  | hnf_pi1 :  forall p T x y, 
+    hnf p (Pair T x y) ->
     forall H, hnf x H -> 
-    hnf (Pi1 (Pair T x y)) H
-  | hnf_pi2 :  forall T x y, 
-    forall H, hnf y H -> 
-    hnf (Pi2 (Pair T x y)) H
-  | hnf_other : forall x, ~ (redex x) -> hnf x x.
+    hnf (Pi1 p) H
+  | hnf_pi2 :  forall p T x y, hnf p (Pair T x y) ->
+    forall H, hnf y H -> hnf (Pi2 p) H
+  | hnf_other : forall x, ~ (exists y, hnf x y /\ y <> x) -> hnf x x.
 
 Lemma hnf_prod : forall U V, hnf (Prod U V) (Prod U V).
 Proof.
@@ -71,7 +103,20 @@ Proof.
   auto.
 Qed.
 
-Lemma hnf_
+Lemma hnf_total : forall x, exists y, hnf x y.
+Proof.
+  induction x.
+
+  exists (Srt s) ; apply hnf_other ; simpl ; auto.
+
+  exists (Ref n) ; apply hnf_other ; simpl ; auto.
+
+  exists (Abs x1 x2) ; apply hnf_other ; simpl ; auto.
+
+  (* App *)
+  induction IHx1.
+  induction x1.
+  exists (Srt s) ; apply hnf_other ; simpl ; auto.
 
 
 
